Fix and verify the third stage of fe25519_mul.

fe25519/fe25519_mul_stage12.v
@@ -5,11 +5,20 @@ From mathcomp Require Import seq .
 Open Scope N_scope.
 Open Scope mqhasm_scope.
 
-Definition fe25519_mul : program :=
+Definition fe25519_mul_stage1 : program :=
 
 let          qtwo :=   QConst (2%Z) in
 let         wsize :=   64%positive in
 let      pow2 x n := QBinop QMul x (QPow qtwo n) in
+
+let concat_shift hi lo w :=       (* (hi.lo) << w *)
+      QBinop QMul (QBinop QAdd (QBinop QMul hi (QPow qtwo wsize)) lo)
+                  (QPow qtwo w) in
+
+let crypto_sign_ed25519_amd64_51_REDMASK51 :=
+                       2251799813685247%Z in (* 0x7FFFFFFFFFFFF from consts *)
+let crypto_sign_ed25519_amd64_51_REDMASK51_width :=
+                       51%positive in        (* 51 bits *)
 
 let            x0 :=   0 in (* *[uint64 *](xp +  0) *)
 let            x1 :=   1 in (* *[uint64 *](xp +  8) *)
@@ -28,7 +37,6 @@ let            z3 :=  13 in (* *[uint64 *](rp + 24) *)
 let            z4 :=  14 in (* *[uint64 *](rp + 32) *)
 let         carry := 999 in
 let           tmp := 998 in
-let          tmp2 := 997 in
 
 let            r0 :=  20 in
 let            r1 :=  21 in
@@ -56,6 +64,10 @@ let       mulx219 :=  54 in
 let       mulx319 :=  55 in
 let       mulx419 :=  56 in
 [::
+      (* # CPU: Intel(R) Xeon(R) CPU X5675 @ 3.07GHz *)
+      (* # RAM: 32GB *)
+      (* # Configuration: -c consts -s *)
+      (* # With Boolector 1.6.0 (-minisat): 620m14.276s *)
       (*  *)
       (* int64 rp *)
       (* int64 xp *)
@@ -130,7 +142,6 @@ let       mulx419 :=  56 in
 
       (*  *)
       (* yp = yp *)
-      (*  *)
       (*  *)
 
       (*   #BEGIN MACRO mul *)
@@ -213,7 +224,7 @@ QSplit mulrdx mulrax (QBinop QMul (QVar mulrax) (QVar y4)) wsize;
 QAssign r4 (QVar mulrax);
 QAssign mulr41 (QVar mulrdx);
       (*  *)
-      (*  *)
+      (*    *)
       (*   mulrax = *[uint64 *](xp + 8) *)
       (*   (uint128) mulrdx mulrax = mulrax * *[uint64 *](yp + 0) *)
       (*   carry? r1 += mulrax *)
@@ -329,7 +340,7 @@ QAssign r1 (QBinop QMul (QVar r1) (QVar mulrax));
 QSplit carry r1 (QVar r1) wsize;
 QAssign mulr11 (QBinop QAdd (QVar mulr11) (QBinop QAdd (QVar mulrdx) (QVar carry)));
       (*  *)
-      (*  *)
+      (*    *)
       (*   mulrax = *[uint64 *](xp + 24) *)
       (*   (uint128) mulrdx mulrax = mulrax * *[uint64 *](yp + 0) *)
       (*   carry? r3 += mulrax *)
@@ -375,7 +386,7 @@ QAssign r2 (QBinop QAdd (QVar r2) (QVar mulrax));
 QSplit carry r2 (QVar r2) wsize;
 QAssign mulr21 (QBinop QAdd (QVar mulr21) (QBinop QAdd (QVar mulrdx) (QVar carry)));
       (*  *)
-      (*  *)
+      (*    *)
       (*   mulrax = *[uint64 *](xp + 32) *)
       (*   (uint128) mulrdx mulrax = mulrax * *[uint64 *](yp + 0) *)
       (*   carry? r4 += mulrax *)
@@ -420,118 +431,18 @@ QAssign mulrax (QVar mulx419);
 QSplit mulrdx mulrax (QBinop QMul (QVar mulrax) (QVar y4)) wsize;
 QAssign r3 (QBinop QAdd (QVar r3) (QVar mulrax));
 QSplit carry r3 (QVar r3) wsize;
-QAssign mulr31 (QBinop QAdd (QVar mulr31) (QBinop QAdd (QVar mulrdx) (QVar carry)));
+QAssign mulr31 (QBinop QAdd (QVar mulr31) (QBinop QAdd (QVar mulrdx) (QVar carry)))
       (*  *)
       (*  *)
+      (*   # assert (mulr01.r0) = x0y0 + 19 * (x4y1 + x3y2 + x2y3 + x1y4) && *)
+      (*   #        (mulr11.r1) = (x1y0 + x0y1) + 19 * (x4y2 + x3y3 + x2y4) && *)
+      (*   #        (mulr21.r2) = (x2y0 + x1y1 + x0y2) + 19 * (x4y3 + x3y4) && *)
+      (*   #        (mulr31.r3) = (x3y0 + x2y1 + x1y2 + x0y3) + 19 * (x4y4) && *)
+      (*   #        (mulr41.r4) = (x4y0 + x3y1 + x2y2 + x1y3 + x0y4) *)
       (*  *)
-      (*  *)
-      (*   mulredmask = *[uint64 *] &crypto_sign_ed25519_amd64_51_REDMASK51 *)
-      (*   mulr01 = (mulr01.r0) << 13 *)
-      (*   r0 &= mulredmask *)
-QSplit tmp r0 (QVar r0) 51%positive;
-QAssign mulr01 (QBinop QAdd (pow2 (QVar mulr01) 13%positive) (QVar tmp));
-      (*   mulr11 = (mulr11.r1) << 13 *)
-      (*   r1 &= mulredmask *)
-      (*   r1 += mulr01 *)
-QSplit tmp r1 (QVar r1) 51%positive;
-QAssign mulr11 (QBinop QAdd (pow2 (QVar mulr11) 13%positive) (QVar tmp));
-QAssign r1 (QBinop QAdd (QVar r1) (QVar mulr01));
-      (*   mulr21 = (mulr21.r2) << 13 *)
-      (*   r2 &= mulredmask *)
-      (*   r2 += mulr11 *)
-QSplit tmp r2 (QVar r2) 51%positive;
-QAssign mulr21 (QBinop QAdd (pow2 (QVar mulr21) 13%positive) (QVar tmp));
-QAssign r2 (QBinop QAdd (QVar r2) (QVar mulr11));
-      (*   mulr31 = (mulr31.r3) << 13 *)
-      (*   r3 &= mulredmask *)
-      (*   r3 += mulr21 *)
-QSplit tmp r3 (QVar r3) 51%positive;
-QAssign mulr31 (QBinop QAdd (pow2 (QVar mulr31) 13%positive) (QVar tmp));
-QAssign r3 (QBinop QAdd (QVar r3) (QVar mulr21));
-      (*   mulr41 = (mulr41.r4) << 13 *)
-      (*   r4 &= mulredmask *)
-      (*   r4 += mulr31 *)
-QSplit tmp r4 (QVar r4) 51%positive;
-QAssign mulr41 (QBinop QAdd (pow2 (QVar mulr41) 13%positive) (QVar tmp));
-QAssign r4 (QBinop QAdd (QVar r4) (QVar mulr31));
-      (*   mulr41 = mulr41 * 19 *)
-QAssign mulr41 (QBinop QMul (QVar mulr41) (QConst 19%Z));
-      (*   r0 += mulr41 *)
-QAssign r0 (QBinop QAdd (QVar r0) (QVar mulr41));
-      (*  *)
-      (*  *)
-      (*  *)
-      (*  *)
-      (*   mult = r0 *)
-      (*   (uint64) mult >>= 51 *)
-      (*   mult += r1 *)
-QAssign mult (QVar r0);
-QSplit mult tmp (QVar mult) (51%positive);
-QAssign mult (QBinop QAdd (QVar mult) (QVar r1));
-      (*   r1 = mult *)
-      (*   (uint64) mult >>= 51 *)
-      (*   r0 &= mulredmask *)
-      (*   mult += r2 *)
-QAssign r1 (QVar mult);
-QSplit mult tmp2 (QVar mult) (51%positive);
-QAssign r0 (QVar tmp);
-QAssign mult (QBinop QAdd (QVar mult) (QVar r2));
-      (*   r2 = mult *)
-      (*   (uint64) mult >>= 51 *)
-      (*   r1 &= mulredmask *)
-      (*   mult += r3 *)
-QAssign r2 (QVar mult);
-QSplit mult tmp (QVar mult) (51%positive);
-QAssign r1 (QVar tmp2);
-QAssign mult (QBinop QAdd (QVar mult) (QVar r3));
-      (*   r3 = mult *)
-      (*   (uint64) mult >>= 51 *)
-      (*   r2 &= mulredmask *)
-      (*   mult += r4 *)
-QAssign r3 (QVar mult);
-QSplit mult tmp2 (QVar mult) (51%positive);
-QAssign r2 (QVar tmp);
-QAssign mult (QBinop QAdd (QVar mult) (QVar r4));
-      (*   r4 = mult *)
-      (*   (uint64) mult >>= 51 *)
-      (*   r3 &= mulredmask *)
-QAssign r4 (QVar mult);
-QSplit mult tmp (QVar mult) (51%positive);
-QAssign r3 (QVar tmp2);
-      (*   mult *= 19 *)
-      (*   r0 += mult *)
-      (*   r4 &= mulredmask *)
-QAssign mult (QBinop QMul (QVar mult) (QConst 19%Z));
-QAssign r0 (QBinop QAdd (QVar r0) (QVar mult));
-QAssign r4 (QVar tmp);
-      (*   #END MACRO mul *)
-
-      (*  *)
-      (* *[uint64 *](rp + 0) = r0 *)
-      (* *[uint64 *](rp + 8) = r1 *)
-      (* *[uint64 *](rp + 16) = r2 *)
-      (* *[uint64 *](rp + 24) = r3 *)
-      (* *[uint64 *](rp + 32) = r4 *)
-QAssign z0 (QVar r0);
-QAssign z1 (QVar r1);
-QAssign z2 (QVar r2);
-QAssign z3 (QVar r3);
-QAssign z4 (QVar r4)
-      (*  *)
-
-      (* c1 =c1_stack *)
-      (* c2 =c2_stack *)
-      (* c3 =c3_stack *)
-      (* c4 =c4_stack *)
-      (* c5 =c5_stack *)
-      (* c6 =c6_stack *)
-      (* c7 =c7_stack *)
-      (*  *)
-
-      (* leave *)
 ] .
 
-Definition fe25519_mul_inputs : VS.t :=
+Definition fe25519_mul_stage1_inputs : VS.t :=
 let            x0 :=   0 in
 let            x1 :=   1 in
 let            x2 :=   2 in
@@ -544,48 +455,83 @@ let            y3 :=   8 in
 let            y4 :=   9 in
 VSLemmas.OP.P.of_list [:: x0; x1; x2; x3; x4; y0; y1; y2; y3; y4].
 
-Definition fe25519_mul_pre : bexp := QTrue.
+Definition fe25519_mul_stage1_pre : bexp := QTrue.
 
-Definition fe25519_mul_post : bexp :=
-let            x0 :=   0 in
-let            x1 :=   1 in
-let            x2 :=   2 in
-let            x3 :=   3 in
-let            x4 :=   4 in
-let            y0 :=   5 in
-let            y1 :=   6 in
-let            y2 :=   7 in
-let            y3 :=   8 in
-let            y4 :=   9 in
+Definition fe25519_mul_stage1_post : bexp :=
+let      pow2 x n := QBinop QMul x (QPow qtwo n) in
+let            x0 :=   0 in (* *[uint64 *](xp +  0) *)
+let            x1 :=   1 in (* *[uint64 *](xp +  8) *)
+let            x2 :=   2 in (* *[uint64 *](xp + 16) *)
+let            x3 :=   3 in (* *[uint64 *](xp + 24) *)
+let            x4 :=   4 in (* *[uint64 *](xp + 32) *)
+let            y0 :=   5 in (* *[uint64 *](yp +  0) *)
+let            y1 :=   6 in (* *[uint64 *](yp +  8) *)
+let            y2 :=   7 in (* *[uint64 *](yp + 16) *)
+let            y3 :=   8 in (* *[uint64 *](yp + 24) *)
+let            y4 :=   9 in (* *[uint64 *](yp + 32) *)
+let            z0 :=  10 in (* *[uint64 *](rp +  0) *)
+let            z1 :=  11 in (* *[uint64 *](rp +  8) *)
+let            z2 :=  12 in (* *[uint64 *](rp + 16) *)
+let            z3 :=  13 in (* *[uint64 *](rp + 24) *)
+let            z4 :=  14 in (* *[uint64 *](rp + 32) *)
+let         carry := 999 in
+let           tmp := 998 in
+
 let            r0 :=  20 in
 let            r1 :=  21 in
 let            r2 :=  22 in
 let            r3 :=  23 in
 let            r4 :=  24 in
+
+let            c0 :=  30 in
+let            c1 :=  31 in
+let            c2 :=  32 in
+let            c3 :=  33 in
+let            c4 :=  34 in
+
+let        mulr01 :=  40 in
+let        mulr11 :=  41 in
+let        mulr21 :=  42 in
+let        mulr31 :=  43 in
+let        mulr41 :=  44 in
+
+let        mulrax :=  50 in
+let        mulrdx :=  51 in
+let          mult :=  52 in
+let    mulredmask :=  53 in
+let       mulx219 :=  54 in
+let       mulx319 :=  55 in
+let       mulx419 :=  56 in
 let        n25519 := 57896044618658097711785492504343953926634992332820282019728792003956564819949%positive in
-QCong
+QEq
   (
     (Radix51.limbs [::QVar x0; QVar x1; QVar x2; QVar x3; QVar x4])
     @*
     (Radix51.limbs [::QVar y0; QVar y1; QVar y2; QVar y3; QVar y4])
   )
-  (Radix51.limbs [::QVar r0; QVar r1; QVar r2; QVar r3; QVar r4])
-  (n25519).
+  (
+    Radix51.limbs [:: QBinop QAdd (QVar r0) (pow2 (QVar mulr01) 64%positive);
+                      QBinop QAdd (QVar r1) (pow2 (QVar mulr11) 64%positive);
+                      QBinop QAdd (QVar r2) (pow2 (QVar mulr21) 64%positive);
+                      QBinop QAdd (QVar r3) (pow2 (QVar mulr31) 64%positive);
+                      QBinop QAdd (QVar r4) (pow2 (QVar mulr41) 64%positive)
+                  ]
+  ).
 
-Definition fe25519_mul_spec :=
-  {| spre := fe25519_mul_pre;
-     sprog := fe25519_mul;
-     spost := fe25519_mul_post |}.
+Definition fe25519_mul_stage1_spec :=
+  {| spre := fe25519_mul_stage1_pre;
+     sprog := fe25519_mul_stage1;
+     spost := fe25519_mul_stage1_post |}.
 
 Add Rec LoadPath "../lib/gbarith/src/" as GBArith.
 Add ML Path "../lib/gbarith/src/".
 From mathcomp Require Import eqtype ssrbool.
 From mQhasm Require Import Verify.
 
-Lemma valid_fe25519_mul : valid_ispec (fe25519_mul_inputs, fe25519_mul_spec).
+Lemma valid_fe25519_mul_stage1 : valid_ispec (fe25519_mul_stage1_inputs, fe25519_mul_stage1_spec).
 Proof.
   Time verify_ispec.
-  (* *)
+  (* nsatz failed after 17753.14s *)
 Qed.
 
 Close Scope mqhasm_scope.
