fe25519/fe25519_mul_stage3-1.v
@@ -1,0 +1,207 @@
+From Coq Require Import ZArith .
+From mQhasm Require Import mQhasm .
+From mathcomp Require Import seq .
+
+Open Scope N_scope.
+Open Scope mqhasm_scope.
+
+Definition fe25519_mul_stage2 : program :=
+
+let          qtwo :=   QConst (2%Z) in
+let         wsize :=   64%positive in
+let      pow2 x n := QBinop QMul x (QPow qtwo n) in
+
+let            x0 :=   0 in (* *[uint64 *](xp +  0) *)
+let            x1 :=   1 in (* *[uint64 *](xp +  8) *)
+let            x2 :=   2 in (* *[uint64 *](xp + 16) *)
+let            x3 :=   3 in (* *[uint64 *](xp + 24) *)
+let            x4 :=   4 in (* *[uint64 *](xp + 32) *)
+let            y0 :=   5 in (* *[uint64 *](yp +  0) *)
+let            y1 :=   6 in (* *[uint64 *](yp +  8) *)
+let            y2 :=   7 in (* *[uint64 *](yp + 16) *)
+let            y3 :=   8 in (* *[uint64 *](yp + 24) *)
+let            y4 :=   9 in (* *[uint64 *](yp + 32) *)
+let            z0 :=  10 in (* *[uint64 *](rp +  0) *)
+let            z1 :=  11 in (* *[uint64 *](rp +  8) *)
+let            z2 :=  12 in (* *[uint64 *](rp + 16) *)
+let            z3 :=  13 in (* *[uint64 *](rp + 24) *)
+let            z4 :=  14 in (* *[uint64 *](rp + 32) *)
+let           tmp := 998 in
+
+let            r0 :=  20 in
+let            r1 :=  21 in
+let            r2 :=  22 in
+let            r3 :=  23 in
+let            r4 :=  24 in
+
+let            c0 :=  30 in
+let            c1 :=  31 in
+let            c2 :=  32 in
+let            c3 :=  33 in
+let            c4 :=  34 in
+
+let        mulr01 :=  40 in
+let        mulr11 :=  41 in
+let        mulr21 :=  42 in
+let        mulr31 :=  43 in
+let        mulr41 :=  44 in
+
+let        mulrax :=  50 in
+let        mulrdx :=  51 in
+let          mult :=  52 in
+let    mulredmask :=  53 in
+let       mulx219 :=  54 in
+let       mulx319 :=  55 in
+let       mulx419 :=  56 in
+[::
+QAssign z0 (QBinop QAdd (QVar r0) (pow2 (QVar mulr01) 64%positive));
+QAssign z1 (QBinop QAdd (QVar r1) (pow2 (QVar mulr11) 64%positive));
+QAssign z2 (QBinop QAdd (QVar r2) (pow2 (QVar mulr21) 64%positive));
+QAssign z3 (QBinop QAdd (QVar r3) (pow2 (QVar mulr31) 64%positive));
+QAssign z4 (QBinop QAdd (QVar r4) (pow2 (QVar mulr41) 64%positive));
+      (*   mulr01 = (mulr01.r0) << 13 *)
+      (*   r0 &= mulredmask *)
+QSplit tmp r0 (QVar r0) 51%positive;
+QAssign mulr01 (QBinop QAdd (pow2 (QVar mulr01) 13%positive) (QVar tmp));
+      (*   mulr11 = (mulr11.r1) << 13 *)
+      (*   r1 &= mulredmask *)
+      (*   r1 += mulr01 *)
+QSplit tmp r1 (QVar r1) 51%positive;
+QAssign mulr11 (QBinop QAdd (pow2 (QVar mulr11) 13%positive) (QVar tmp));
+QAssign r1 (QBinop QAdd (QVar r1) (QVar mulr01));
+      (*   mulr21 = (mulr21.r2) << 13 *)
+      (*   r2 &= mulredmask *)
+      (*   r2 += mulr11 *)
+QSplit tmp r2 (QVar r2) 51%positive;
+QAssign mulr21 (QBinop QAdd (pow2 (QVar mulr21) 13%positive) (QVar tmp));
+QAssign r2 (QBinop QAdd (QVar r2) (QVar mulr11));
+      (*   mulr31 = (mulr31.r3) << 13 *)
+      (*   r3 &= mulredmask *)
+      (*   r3 += mulr21 *)
+QSplit tmp r3 (QVar r3) 51%positive;
+QAssign mulr31 (QBinop QAdd (pow2 (QVar mulr31) 13%positive) (QVar tmp));
+QAssign r3 (QBinop QAdd (QVar r3) (QVar mulr21));
+      (*   mulr41 = (mulr41.r4) << 13 *)
+      (*   r4 &= mulredmask *)
+      (*   r4 += mulr31 *)
+QSplit tmp r4 (QVar r4) 51%positive;
+QAssign mulr41 (QBinop QAdd (pow2 (QVar mulr41) 13%positive) (QVar tmp));
+QAssign r4 (QBinop QAdd (QVar r4) (QVar mulr31));
+      (*   mulr41 = mulr41 * 19 *)
+QAssign mulr41 (QBinop QMul (QVar mulr41) (QConst 19%Z));
+      (*   r0 += mulr41 *)
+QAssign r0 (QBinop QAdd (QVar r0) (QVar mulr41))
+      (*  *)
+      (*  *)
+      (*  *)
+      (*  *)
+] .
+
+Definition fe25519_mul_stage2_inputs : VS.t :=
+let            x0 :=   0 in (* *[uint64 *](xp +  0) *)
+let            x1 :=   1 in (* *[uint64 *](xp +  8) *)
+let            x2 :=   2 in (* *[uint64 *](xp + 16) *)
+let            x3 :=   3 in (* *[uint64 *](xp + 24) *)
+let            x4 :=   4 in (* *[uint64 *](xp + 32) *)
+let            y0 :=   5 in (* *[uint64 *](yp +  0) *)
+let            y1 :=   6 in (* *[uint64 *](yp +  8) *)
+let            y2 :=   7 in (* *[uint64 *](yp + 16) *)
+let            y3 :=   8 in (* *[uint64 *](yp + 24) *)
+let            y4 :=   9 in (* *[uint64 *](yp + 32) *)
+let            z0 :=  10 in (* *[uint64 *](rp +  0) *)
+let            z1 :=  11 in (* *[uint64 *](rp +  8) *)
+let            z2 :=  12 in (* *[uint64 *](rp + 16) *)
+let            z3 :=  13 in (* *[uint64 *](rp + 24) *)
+let            z4 :=  14 in (* *[uint64 *](rp + 32) *)
+let         carry := 999 in
+let           tmp := 998 in
+let            r0 :=  20 in
+let            r1 :=  21 in
+let            r2 :=  22 in
+let            r3 :=  23 in
+let            r4 :=  24 in
+let            c0 :=  30 in
+let            c1 :=  31 in
+let            c2 :=  32 in
+let            c3 :=  33 in
+let            c4 :=  34 in
+let        mulr01 :=  40 in
+let        mulr11 :=  41 in
+let        mulr21 :=  42 in
+let        mulr31 :=  43 in
+let        mulr41 :=  44 in
+let        mulrax :=  50 in
+let        mulrdx :=  51 in
+let          mult :=  52 in
+let    mulredmask :=  53 in
+let       mulx219 :=  54 in
+let       mulx319 :=  55 in
+let       mulx419 :=  56 in
+VSLemmas.OP.P.of_list [:: mulr01; r0; mulr11; r1; mulr21; r2; mulr31; r3; mulr41; r4].
+
+Definition fe25519_mul_stage2_pre : bexp := QTrue.
+
+Definition fe25519_mul_stage2_post : bexp :=
+let            x0 :=   0 in (* *[uint64 *](xp +  0) *)
+let            x1 :=   1 in (* *[uint64 *](xp +  8) *)
+let            x2 :=   2 in (* *[uint64 *](xp + 16) *)
+let            x3 :=   3 in (* *[uint64 *](xp + 24) *)
+let            x4 :=   4 in (* *[uint64 *](xp + 32) *)
+let            y0 :=   5 in (* *[uint64 *](yp +  0) *)
+let            y1 :=   6 in (* *[uint64 *](yp +  8) *)
+let            y2 :=   7 in (* *[uint64 *](yp + 16) *)
+let            y3 :=   8 in (* *[uint64 *](yp + 24) *)
+let            y4 :=   9 in (* *[uint64 *](yp + 32) *)
+let            z0 :=  10 in (* *[uint64 *](rp +  0) *)
+let            z1 :=  11 in (* *[uint64 *](rp +  8) *)
+let            z2 :=  12 in (* *[uint64 *](rp + 16) *)
+let            z3 :=  13 in (* *[uint64 *](rp + 24) *)
+let            z4 :=  14 in (* *[uint64 *](rp + 32) *)
+let         carry := 999 in
+let           tmp := 998 in
+let            r0 :=  20 in
+let            r1 :=  21 in
+let            r2 :=  22 in
+let            r3 :=  23 in
+let            r4 :=  24 in
+let            c0 :=  30 in
+let            c1 :=  31 in
+let            c2 :=  32 in
+let            c3 :=  33 in
+let            c4 :=  34 in
+let        mulr01 :=  40 in
+let        mulr11 :=  41 in
+let        mulr21 :=  42 in
+let        mulr31 :=  43 in
+let        mulr41 :=  44 in
+let        mulrax :=  50 in
+let        mulrdx :=  51 in
+let          mult :=  52 in
+let    mulredmask :=  53 in
+let       mulx219 :=  54 in
+let       mulx319 :=  55 in
+let       mulx419 :=  56 in
+let        n25519 := 57896044618658097711785492504343953926634992332820282019728792003956564819949%positive in
+QCong
+  (Radix51.limbs [::QVar z0; QVar z1; QVar z2; QVar z3; QVar z4])
+  (Radix51.limbs [::QVar r0; QVar r1; QVar r2; QVar r3; QVar r4])
+  (n25519).
+
+Definition fe25519_mul_stage2_spec :=
+  {| spre := fe25519_mul_stage2_pre;
+     sprog := fe25519_mul_stage2;
+     spost := fe25519_mul_stage2_post |}.
+
+Add Rec LoadPath "../lib/gbarith/src/" as GBArith.
+Add ML Path "../lib/gbarith/src/".
+From mathcomp Require Import eqtype ssrbool.
+From mQhasm Require Import Verify.
+
+Lemma valid_fe25519_mul_stage2 : valid_ispec (fe25519_mul_stage2_inputs, fe25519_mul_stage2_spec).
+Proof.
+  Time verify_ispec.
+  (* 52.34s *)
+Qed.
+
+Close Scope mqhasm_scope.
+Close Scope N_scope.
